fix (Otway-Rees): third protocol step is now verified by FStar
FStar seems to have a problem verifying the code if match statements are not nested
but instead, the result is "piped" to the outter scope. Thus, it was necessary
to rewrite the third step such that match statements are nested. Code is now
verified w/o problems.

otway-rees/OYRS.Protocol.fst
@@ -139,53 +139,62 @@ let server_send_msg_3 srv msg2_idx =
 
       // decrypt parts of message encrypted by initiator and responder, respectively
       let c_ev_a:msg oyrs_global_usage now public = c_ev_a in
-      let ser_ev_a = (match aead_dec #oyrs_global_usage #now #(get_label oyrs_key_usages k_as) k_as (string_to_bytes #oyrs_global_usage #now "iv") c_ev_a (string_to_bytes #oyrs_global_usage #now "ev1") with
-      | Success ser_ev_a -> ser_ev_a
-      | Error e -> error ("srv_send_m3: decryption of initiator part failed: " ^ e)) in
+      match aead_dec #oyrs_global_usage #now #(get_label oyrs_key_usages k_as) k_as (string_to_bytes #oyrs_global_usage #now "iv") c_ev_a (string_to_bytes #oyrs_global_usage #now "ev1") with
+      | Success ser_ev_a -> (
+        let c_ev_b:msg oyrs_global_usage now public = c_ev_b in
+        match aead_dec #oyrs_global_usage #now #(get_label oyrs_key_usages k_bs) k_bs (string_to_bytes #oyrs_global_usage #now "iv") c_ev_b (string_to_bytes #oyrs_global_usage #now "ev1") with
+        | Success ser_ev_b -> (
+          // parse the decrypted message parts
+          match parse_encval ser_ev_a with
+          | Success (EncMsg1 n_a c_a a_a b_a) -> (
+            match parse_encval ser_ev_b with
+            | Success (EncMsg2 n_b c_b a_b b_b) -> (
+              if c_a <> c_b || a_a <> a_b || b_a <> b_b then error "srv_send_m3: encrypted parts of initiator and responder do not match"
+              else
+                // generate shared conversation key between initiator and responder
+                let (|_,k_ab|) = rand_gen #oyrs_preds (readers [P srv; P a; P b]) (aead_usage "sk_i_r") in
 
-      let c_ev_b:msg oyrs_global_usage now public = c_ev_b in
-      let ser_ev_b = (match aead_dec #oyrs_global_usage #now #(get_label oyrs_key_usages k_bs) k_bs (string_to_bytes #oyrs_global_usage #now "iv") c_ev_b (string_to_bytes #oyrs_global_usage #now "ev1") with
-                     | Success ser_ev_b -> ser_ev_b
-                     | Error e -> error ("srv_send_m3: decryption of responder part failed: " ^ e)) in
+                // create and send third message
+                let ev3_i = EncMsg3_I n_a k_ab in
+                let now = global_timestamp () in
+                includes_can_flow_lemma now [P srv; P a; P b] [P a; P srv];
+                let ser_ev3_i = serialize_encval now ev3_i (get_label oyrs_key_usages k_as) in
+                let c_ev3_i = aead_enc #oyrs_global_usage #now #(get_label oyrs_key_usages k_as) k_as (string_to_bytes #oyrs_global_usage #now "iv") ser_ev3_i (string_to_bytes #oyrs_global_usage #now "ev3_i") in
 
-      // parse the decrypted message parts
-      let (EncMsg1 n_a c_a a_a b_a) = (match parse_encval ser_ev_a with
-                                      | Success (EncMsg1 n_a c_a a_a b_a) -> (EncMsg1 n_a c_a a_a b_a)
-                                      | _ -> error "srv_send_m3: wrong initiator encval") in
+                let ev3_r = EncMsg3_R n_b k_ab in
+                let now = global_timestamp () in
+                includes_can_flow_lemma now [P srv; P a; P b] [P b; P srv];
+                let ser_ev3_r = serialize_encval now ev3_r (get_label oyrs_key_usages k_bs) in
+                let c_ev3_r = aead_enc #oyrs_global_usage #now #(get_label oyrs_key_usages k_bs) k_bs (string_to_bytes #oyrs_global_usage #now "iv") ser_ev3_r (string_to_bytes #oyrs_global_usage #now "ev3_r") in
 
-      let (EncMsg2 n_b c_b a_b b_b) = (match parse_encval ser_ev_b with
-                                      | Success (EncMsg2 n_b c_b a_b b_b) -> (EncMsg1 n_b c_b a_b b_b)
-                                      | _ -> error "srv_send_m3: wrong responder encval") in
+                let msg3 = Msg3 c c_ev3_i c_ev3_r in
+                let now = global_timestamp () in
+                let ser_msg3 = serialize_msg now msg3 in
 
-      if c_a <> c_b || a_a <> a_b || b_a <> b_b then error "srv_send_m3: encrypted parts of initiator and responder do not match"
-      else
-        // generate shared conversation key between initiator and responder
-        let (|_,k_ab|) = rand_gen #oyrs_preds (readers [P srv; P a; P b]) (aead_usage "sk_i_r") in
+                let send_m3_idx = send #oyrs_preds #now srv b ser_msg3 in
 
-        // create and send third message
-        let ev3_i = EncMsg3_I n_a k_ab in
-        let now = global_timestamp () in
-        let ser_ev3_i = serialize_encval now ev3_i (get_label oyrs_key_usages k_as) in
-        let c_ev3_i = aead_enc #oyrs_global_usage #now #(get_label oyrs_key_usages k_as) k_as (string_to_bytes #oyrs_global_usage #now "iv") ser_ev3_i (string_to_bytes #oyrs_global_usage #now "ev3_i") in
+                // store server session
+                let new_sess_idx = new_session_number #oyrs_preds srv in
+                let st_srv_sent_m3 = AuthServerSentMsg3 a b c n_a n_b k_ab in
+                let now = global_timestamp () in
+                assert(is_publishable oyrs_global_usage now c);
+                assert(is_labeled oyrs_global_usage now k_as (readers [P a; P srv]));
+                assert(is_labeled oyrs_global_usage now k_bs (readers [P b; P srv]));
+                assert(is_msg oyrs_global_usage now n_a (get_label oyrs_key_usages k_as));
+                assert(is_msg oyrs_global_usage now n_b (get_label oyrs_key_usages k_bs));
+                includes_can_flow_lemma now [P a; P srv] [P srv];
+                includes_can_flow_lemma now [P b; P srv] [P srv];
+                let ser_st = serialize_session_st now srv new_sess_idx 0 st_srv_sent_m3 in
+                new_session #oyrs_preds #now srv new_sess_idx 0 ser_st;
 
-        let ev3_r = EncMsg3_R n_b k_ab in
-        let now = global_timestamp () in
-        let ser_ev3_r = serialize_encval now ev3_r (get_label oyrs_key_usages k_bs) in
-        let c_ev3_r = aead_enc #oyrs_global_usage #now #(get_label oyrs_key_usages k_bs) k_bs (string_to_bytes #oyrs_global_usage #now "iv") ser_ev3_r (string_to_bytes #oyrs_global_usage #now "ev3_r") in
-
-        let msg3 = Msg3 c c_ev3_i c_ev3_r in
-        let now = global_timestamp () in
-        let ser_msg3 = serialize_msg now msg3 in
-
-        let send_m3_idx = send #oyrs_preds #now srv b ser_msg3 in
-
-        // store server session
-        let new_sess_idx = new_session_number #oyrs_preds srv in
-        let st_srv_sent_m3 = AuthServerSentMsg3 a b c n_a n_b k_ab in
-        let now = global_timestamp () in
-        let ser_st = serialize_session_st now srv new_sess_idx 0 st_srv_sent_m3 in
-        new_session #oyrs_preds #now srv new_sess_idx 0 ser_st;
-
-        (new_sess_idx, send_m3_idx)
+                (new_sess_idx, send_m3_idx)
+            )
+            | _ -> error "srv_send_m3: wrong responder encval"
+          )
+          | _ -> error "srv_send_m3: wrong initiator encval"
+        )
+        | Error e -> error ("srv_send_m3: decryption of responder part failed: " ^ e)
+      )
+      | Error e -> error ("srv_send_m3: decryption of initiator part failed: " ^ e)
   )
   | _ -> error "srv_send_m3: wrong message"
